StarCombinator.Base.fst
@@ -1,51 +1,35 @@
 module StarCombinator.Base
 
 open StarCombinator.Core
+open StarCombinator.Operators
 open FStar.String
 open FStar.Char
 
+module H = StarCombinator.Helpers
 module C = StarCombinator.Constants
 module L = FStar.List.Tot.Base
 module M = FStar.Mul
 
-private
-let undefErr p0 p1 = ParserRes None (undefErr p0 p1 "undef")
-
-(** if ch is matched, it output symb  **)
-let satisfy (f: char -> bool) : parser char
-    = fun src pos -> if pos >= FStar.String.length src
-                  then undefErr (if pos = 0 then 0 else pos-1) pos
-                  else (
-                     let current = get src pos in
-                     if f current
-                     then ParserRes (Some (pos+1, current)) noError
-                     else undefErr pos (pos+1)
-                  )
-
-private
-let rec lst_contains (#a:eqtype)  (x: a) (l: list a) = match l with
-  | [] -> false | h::t -> x = h || lst_contains x t
-
 let exact (exactChar: char) : parser char
-    = satisfy (fun c -> c = exactChar) <?> "expected '" ^ string_of_list [exactChar] ^ "'"
+    = satisfy_char (fun c -> c = exactChar) <?> "expected '" ^ string_of_list [exactChar] ^ "'"
+
+private
+let showRange r = String.concat "" (L.map (fun x -> match x with
+                                               | '\n' -> "\\n"
+                                               | '\t' -> "\\t"
+                                               |  ch  -> string_of_list [ch]
+                                         ) r)
 
 let oneOf (possibles: list char): parser char
-    = satisfy (fun c -> lst_contains c possibles) <?> "expected something in the range [" ^ string_of_list possibles ^ "]"
+    = satisfy_char (fun c -> H.lst_contains c possibles) <?> "expected something in the range [" ^ showRange possibles ^ "]"
 
 let noneOf (possibles: list char): parser char
-    = satisfy (fun c -> not (lst_contains c possibles)) <?> "expected something out of the range ["^string_of_list possibles^"]"
-
-(** Identity for parsers, in a sense **)
-let match_empty #a (symb: a) : parser a = fun _ pos -> ParserRes (Some (pos, symb)) noError
-
-
-//let space = oneOf C.isSpaceChar
+    = satisfy_char (fun c -> not (H.lst_contains c possibles)) <?> "expected something out of the range ["^showRange possibles^"]"
 
 let space = oneOf ('\n'::C.isSpaceChar)
 
  (* zero one or more spaces *)
 let spaces: parser unit = fp (fun _ -> ()) (many space)
-
 
 let newline = fp (fun _ -> ()) (exact '\n')
 let crlf = fp (fun _ -> ()) (exact '\r' <*> newline)
@@ -59,17 +43,17 @@ let upper = oneOf C.upperCaseCharList
 
 let digit = oneOf C.digitList
 
-let charClass (l:list char {~(l == [])}): parser char = choice (L.map exact l)
+//let charClass (l:list char {~(l == [])}): parser char = choice (L.map exact l)
 
 let digit_num : parser (n: nat{n <= 9}) = 
   let convert (c:char): (n: nat{n <= 9}) = match c with
               | '1' -> 1 | '2' -> 2 | '3' -> 3 | '4' -> 4 | '5' -> 5
               | '6' -> 6 | '7' -> 7 | '8' -> 8 | '9' -> 9 |  _  -> 0 in
-  fp convert (charClass C.digitList) <?> "expected digit"
+  fp convert (oneOf C.digitList) <?> "expected digit"
 
-let notLetter = (fp (fun _ -> ' ') eof <||> satisfy (fun c -> lst_contains c C.anyCaseCharList)) <?> "expected something different than a letter"
+let notLetter = (satisfy_char (fun c -> H.lst_contains c C.anyCaseCharList) <|> fp (fun _ -> ' ') eof) <?> "expected something different than a letter"
 
-let letter = charClass C.anyCaseCharList <?> "expected letter"
+let letter = oneOf C.anyCaseCharList <?> "expected letter"
 
 let natural_number : parser nat =
   let rec convert (c:list (n: nat{n <= 9})): nat = match c with
@@ -82,17 +66,20 @@ let number: parser int = fp (fun ((m, n): (option char*nat)) -> match m with | S
                        (maybe (exact '-') <*> natural_number) <?> "expected number"
 
 
-let alphaNum = charClass (C.digitList @ C.anyCaseCharList) <?> "expected alphanumeric"
+let alphaNum = oneOf (C.digitList @ C.anyCaseCharList) <?> "expected alphanumeric"
 
-let hexDigit = charClass (C.digitList @ list_of_string "ABCDEFabcdef") <?> "expected hex digit"
+let hexDigit = oneOf (C.digitList @ list_of_string "ABCDEFabcdef") <?> "expected hex digit"
+
+let sequence #a (lp: list (parser a) {~(lp == [])}) = let (hd::lp) = lp in
+    L.fold_left (fun (acc: parser (list a)) (y: parser a) -> fp (fun (l, v) -> l @ [v]) (acc <*> y)) (fp (fun x -> [x]) hd) lp
 
 let exact_string (str:string{str <> ""}): parser string = fp string_of_list (sequence #char (admitP(list_of_string str <> []); L.map exact (list_of_string str))) <?> "expected the exact string \""^str^"\""
 
-let string_satisfy (fchar: char -> bool): parser string = fp string_of_list (many1 (satisfy fchar)) <?> "expected some string maching some predicate"
+let string_satisfy (fchar: char -> bool): parser string = fp string_of_list (many1 (satisfy_char fchar)) <?> "expected some string maching some predicate"
 
-let word: parser string = (string_satisfy (fun c -> lst_contains c C.anyCaseCharList) <<*> notFollowedBy letter) <?> "expected a word"
+let word: parser string = (string_satisfy (fun c -> H.lst_contains c C.anyCaseCharList) <<*> notFollowedBy letter) <?> "expected a word"
 
-let keyword str: parser unit = fp (fun _ -> ()) (spaces <*> exact_string str <*> spaces <<*> notFollowedBy letter) <?> "expected the keyword "^str
+let keyword str: parser unit = fp (fun _ -> ()) (ptry (spaces <*> exact_string str) <*> spaces <<*> notFollowedBy letter) <?> "expected the keyword "^str
 
 let keywords (lstr: list string{lstr<>[]}): parser unit = fp (fun _ -> ()) (sequence #string (admit(); L.map (fun s -> spaces <*>> exact_string s) lstr) <*> spaces) <?> "expected the keywords " ^ (String.concat " " lstr)
 
@@ -102,6 +89,12 @@ let wrapspace p = spaces <*>> p <<*> spaces
 
 let match_boolean_litterate = ((fp (fun x -> true) (exact_string "true")) <|> (fp (fun x -> false) (exact_string "false"))) <?> "expected false or true"
 
+let between l r i = l <*>> i <<*> r
+
 let between_kwd l r i = between (keyword l) (keyword r) i <?> "expected something of the form \""^l^" ... "^r^"\""
 
+let sepBy1 i s = (fun (v,l) -> v::l) `fp` i <*> (many (s <*> i))
+let sepBy i s = ptry ((fun (v,l) -> v::l) `fp` (i <*> (many (s <*>> i)))) <|> fp (fun x -> [x]) i
+
 let match_list l r s i = between_kwd l r (sepBy i (keyword s)) <?> "expected a list \""^l^" ... "^s^" ... "^r^"\""
+
