StarCombinator.Examples.While.fst
@@ -2,6 +2,8 @@ module StarCombinator.Examples.While
 
 open StarCombinator
 
+module L = FStar.List.Tot.Base
+
 type lAExp =
   | LAExpLitt : int -> lAExp
   | LAExpVar  : string -> lAExp
@@ -27,31 +29,75 @@ type lFakeInstr =
   | LFakeInstrFunDef : funFakeDef -> lFakeInstr
 and funFakeDef = | FunFakeDef : string -> list string -> lFakeInstr -> funFakeDef
 
+let rec lAExpToString x = match x with
+  | LAExpLitt  a   -> string_of_int a//int -> lAExp
+  | LAExpVar   a   -> a//string -> lAExp
+  | LAExpPlus  a b -> "("^lAExpToString a ^ "+" ^ lAExpToString b^")"//lAExp  -> lAExp -> lAExp 
+  | LAExpMinus a b -> "("^lAExpToString a ^ "-" ^ lAExpToString b^")"//lAExp  -> lAExp -> lAExp 
+  | LAExpMult  a b -> "("^lAExpToString a ^ "*" ^ lAExpToString b^")"//lAExp  -> lAExp -> lAExp
+  | LAExpDiv   a b -> "("^lAExpToString a ^ "/" ^ lAExpToString b^")"//lAExp  -> lAExp -> lAExp
+
+let rec lBExpToString x = match x with
+  | LBExpLitt a   -> (if a then "true" else "false") //: bool -> lBExp
+  | LBExpNot  a   -> "~"^lBExpToString a //: lBExp -> lBExp
+  | LBExpAnd  a b -> "("^lBExpToString a ^ "&&" ^ lBExpToString b^")" //: lBExp -> lBExp -> lBExp
+  | LBExpOr   a b -> "("^lBExpToString a ^ "||" ^ lBExpToString b^")" //: lBExp -> lBExp -> lBExp
+  | LBExpEq   a b -> "("^lAExpToString a ^ "==" ^ lAExpToString b^")" //: lAExp -> lAExp -> lBExp
+  | LBExpLe   a b -> "("^lAExpToString a ^ "<=" ^ lAExpToString b^")" //: lAExp -> lAExp -> lBExp
+
+let rec lInstrAssignableToString x = match x with
+  | AssignLAExp a -> lAExpToString a
+  | AssignCall  fn args -> fn ^ "(" ^ String.concat ", " (L.map lAExpToString args) ^ ")"
+
+let rec lFakeInstrToString x = match x with
+  | LFakeInstrAssign a b -> a ^ " = " ^ lInstrAssignableToString b //: string -> lInstrAssignable -> lFakeInstr
+  | LFakeInstrSkip       -> "SKIP"//: lFakeInstr
+  | LFakeInstrSeq    a b -> lFakeInstrToString a^";"^lFakeInstrToString b//: lFakeInstr -> lFakeInstr -> lFakeInstr
+  | LFakeInstrIf   c a b -> "if (" ^ lBExpToString c ^ ") { " ^ lFakeInstrToString a ^ " } else { " ^lFakeInstrToString b^" }" //: lBExp -> lFakeInstr -> lFakeInstr -> lFakeInstr
+  | LFakeInstrWhile  c a -> "while (" ^ lBExpToString c ^ ") { " ^ lFakeInstrToString a ^" }"//: lBExp -> lFakeInstr -> lFakeInstr
+  | LFakeInstrFunDef (FunFakeDef fn args _) -> "FunDef(TODO)"//: funFakeDef -> lFakeInstr
 
 private
 let uncurry f x = let (l,r) = x in f l r
 private
 let uncurry3 f x = let ((a,b),c) = x in f a b c
 
+let op_apply = (fun (l, mb) -> match mb with
+          | None -> l
+          | Some (op, r) -> op l r
+          )
+
 let aexp_parser: parser lAExp =
-  let rec no_rec (): parser lAExp = fp LAExpLitt number <||> fp LAExpVar word
-                   <||> (keyword "(" <*>> (admitP (() << ()); delayMe h') <<*> keyword ")")
+  let rec no_rec (): parser lAExp =
+          between_kwd "(" ")" (admitP (()<<()); delayMe h')
+      <|> fp LAExpLitt number
+      <|> fp LAExpVar word
+      
   and h' (): parser lAExp = admitP (() << ()); let h = delayMe h' in
-         no_rec () <||> fp (uncurry LAExpPlus)  (no_rec () <<*> ckwd '+' <*> h)
-                   <||> fp (uncurry LAExpMinus) (no_rec () <<*> ckwd '-' <*> h)
-                   <||> fp (uncurry LAExpMult)  (no_rec () <<*> ckwd '*' <*> h)
-                   <||> fp (uncurry LAExpDiv)  (no_rec () <<*> ckwd '/' <*> h)
+      op_apply @<< (
+            no_rec ()
+          <*> maybe ((
+                (LAExpPlus *<< keyword "+") <|> (LAExpMinus *<< keyword "-")
+            <|> (LAExpMult *<< keyword "*") <|> (LAExpDiv *<< keyword "/")
+          ) <*> h)
+        )      
   in wrapspace (h' ())
 
 let bexp_parser: parser lBExp =
-  let rec no_rec (): parser lBExp = fp LBExpLitt (wrapspace match_boolean_litterate)
-           <||> fp (uncurry LBExpEq) (aexp_parser <<*> exact_string "=="  <*> aexp_parser)
-           <||> fp (uncurry LBExpLe) (aexp_parser <<*> exact_string "<="  <*> aexp_parser)
-           <||> fp LBExpNot (exact '~' <*>> (admitP (() << ()); delayMe no_rec))
-           <||> (between (keyword "(") (keyword ")") (delayMe h'))
-  and h' (): parser lBExp = admitP (() << ()); let h = delayMe h' in
-    no_rec () <||> fp (uncurry LBExpAnd) (no_rec () <<*> exact_string "&&" <*> h)
-              <||> fp (uncurry LBExpOr)  (no_rec () <<*> exact_string "||" <*> h)
+  let rec no_rec (): parser lBExp = admitP (() << ()); let nr = delayMe no_rec in
+          (LBExpNot @<< (keyword "~" <*>> nr))
+      <|> ptry (LBExpLitt true  *<< keyword "true" <|> LBExpLitt false *<< keyword "false")
+      <|> ptry (between (keyword "(") (keyword ")") (delayMe h'))
+      <|> ptry (fp (fun ((l, op), r) -> op l r)
+        (aexp_parser <*> (
+           (LBExpEq *<< keyword "==") <|> (LBExpLe *<< keyword "<=")
+        ) <*> aexp_parser))
+  and h' (): parser lBExp =   admitP (() << ()); let h = delayMe h' in
+          op_apply @<<
+          (no_rec () <*> maybe (
+                ((LBExpAnd *<< keyword "&&") <|> (LBExpOr *<< keyword "||"))
+            <*> h
+          ))
   in wrapspace (h' ())
 
 let rec lFakeInstrIsWF prog toplevel = match prog with 
@@ -60,39 +106,53 @@ let rec lFakeInstrIsWF prog toplevel = match prog with
   | LFakeInstrWhile _ a -> lFakeInstrIsWF a false
   | LFakeInstrFunDef (FunFakeDef _ _ a) -> if toplevel then lFakeInstrIsWF a false else false 
   | _ -> true
+
 type lFakeInstrWF = r:lFakeInstr {lFakeInstrIsWF r true}
 
-let hAssignCall var fName args = LFakeInstrAssign var (AssignCall fName args)
-let hAssignExp var exp = LFakeInstrAssign var (AssignLAExp exp) 
+//let hAssignCall (var fName args = 
+//let hAssignExp (var, exp) = LFakeInstrAssign var (AssignLAExp exp) 
+
+let hAssign (var, eith) = match eith with
+    | Inl (fName, args) -> LFakeInstrAssign var (AssignCall fName args)
+    | Inr exp -> LFakeInstrAssign var (AssignLAExp exp) 
 
 let match_comment: parser string = spaces <*>> keyword "//" <*>> string_satisfy (fun x -> x <> '\n')
 let match_comments: parser (list string) = fp (fun x -> match x with | Some x -> x | None -> []) (maybe (many match_comment))
 
+let hIf ((cond, body0), body1) = LFakeInstrIf cond body0 body1
+let hWhile (cond, body) = LFakeInstrWhile cond body
+let hFunction ((str,args),body) = LFakeInstrFunDef (FunFakeDef str args body)
+
+
 let lFakeInstr_parser: parser (r:lFakeInstr) =
    let z #a (arg:parser a) = arg <<*> match_comments in
-   let rec no_rec (tl:bool): parser (r:lFakeInstr) = admitP (() << ()); z (
-           fp (uncurry hAssignExp) (word <<*> keyword "=" <*> aexp_parser)
-       <||> fp (uncurry3 hAssignCall) (word <<*> keyword "="
-              <*> word <*> match_list "(" ")" "," aexp_parser)
-       <||> fp (fun _ -> LFakeInstrSkip) (exact_string "SKIP")
-       <||> fp (uncurry3 LFakeInstrIf) (
-                  ((keywords ["if"; "("] <*>> bexp_parser) <<*> keywords [")"; "{"])
-              <*> ((delayMe (h' false)) <<*> keywords ["}";"else";"{"])
-              <*> ((delayMe (h' false)) <<*> keyword "}")
-           )
-       <||> fp (fun ((str,args),body) -> LFakeInstrFunDef (FunFakeDef str args body)) (
-                  (keyword "function" <*>> word <*> 
-                    (match_list "(" ")" "," word)
-                    <<*> keyword "{")
-              <*> (delayMe (h' false) <<*> keyword "}")
-           )       
-       <||> fp (uncurry LFakeInstrWhile) (
-                  ((keywords ["while";"("] <*>> bexp_parser) <<*> keywords [")";"{"])
-              <*> ((delayMe (h' false)) <<*> keyword "}")
-           ))
-   and h' (tl:bool) (): parser (r:lFakeInstr) = admitP (() << ()); let h = delayMe (h' tl) in
-     z (
-       no_rec tl <||> fp (uncurry LFakeInstrSeq) (no_rec tl <<*> keyword ";" <*> (match_comments <*>> h))
-                 <||> (no_rec tl <<*> keyword ";")
+   let rec no_rec (tl:bool): parser (r:lFakeInstr) = admitP (() << ()); let nr tl = delayMe (fun () -> no_rec tl) in z (
+       ( hIf @<<
+         ((keywords ["if"; "("] <*>> bexp_parser <<*> keywords [")";"{"]) <*>
+           (nr false <<*> keywords ["}";"else";"{"]) <*>
+           (nr false <<*> keyword "}"))
+       )
+   <|> ( hWhile @<< (
+                (keywords ["while"; "("] <*>> bexp_parser <<*> keywords [")";"{"])
+            <*> (nr false <<*> keyword "}")
+            )
+       )
+   <|> ( hFunction @<< (
+                   (keyword "function" <*>> word)
+               <*> (match_list "(" ")" "," word <<*> keyword "{")
+               <*> (nr false <<*> keyword "}")
+               )
+       )
+   <|> (LFakeInstrSkip *<< keyword "SKIP")
+   <|> (hAssign @<< (word <<*> keyword "=" <*> (
+             ptry (word <*> match_list "(" ")" "," aexp_parser)
+         </> aexp_parser
+       )))
+   )
+   and h' (tl:bool) (): parser (r:lFakeInstr) = admitP (() << ()); let h = delayMe (h' tl) in z (
+       (fun (s1, s2) -> match s2 with
+                     | None    -> s1
+                     | Some s2 -> LFakeInstrSeq s1 s2
+       ) @<< (no_rec tl <*> maybe (keyword ";" <*>> (match_comments <*>> h)))
      )
    in wrapspace (h' true ())
